Linglib.lean
@@ -2879,6 +2879,7 @@ import Linglib.Syntax.Minimalist.SyntacticObject.Replace
 import Linglib.Syntax.Minimalist.SyntacticObject.Selection
 import Linglib.Syntax.Minimalist.SyntacticObject.Subterm
 import Linglib.Syntax.Minimalist.Theta.Basic
+import Linglib.Syntax.Minimalist.Theta.Realize
 import Linglib.Syntax.Minimalist.Verbal.Applicative
 import Linglib.Syntax.Minimalist.Verbal.Aspect
 import Linglib.Syntax.Minimalist.Verbal.Decomposition
